Cleanup and document the main proof idea for endpoint_choiceProof

projection/proofs/endpointPropsScript.sml
@@ -2,6 +2,52 @@ open preamble endpointSemanticsTheory endpointLangTheory;
 
 val _ = new_theory "endpointProps"
 
+(* todo: lemmas that have nothing to do with endpointLang, move? *)
+val RTC_SANDWICH = Q.store_thm("RTC_SANDWICH",
+  `!R a b c d. R^* a b /\ R b c /\ R^* c d ==> R^* a d`,
+  metis_tac[RTC_RTC,RTC_SINGLE])
+
+val INDEX_FIND_normalize = Q.store_thm("INDEX_FIND_normalize",
+  `!l n. OPTION_MAP SND (INDEX_FIND n f l) = OPTION_MAP SND (INDEX_FIND 0 f l)`,
+  Induct_on `l` >> rpt strip_tac >> rw[INDEX_FIND_def]);
+
+val INDEX_FIND_normalize' = Q.store_thm("INDEX_FIND_normalize'",
+  `!l n. (INDEX_FIND n f l = NONE) = (INDEX_FIND 0 f l = NONE)`,
+  Induct_on `l` >> rpt strip_tac >> rw[INDEX_FIND_def]);
+
+val INDEX_FIND_normalize'' = Q.store_thm("INDEX_FIND_normalize''",
+  `!n f l z. (INDEX_FIND (SUC n) f l = SOME z) = (FST z > 0 /\ INDEX_FIND n f l = SOME (FST z - 1, SND z))`,
+  Induct_on `l` >> rpt strip_tac
+  >> rw[INDEX_FIND_def,EQ_IMP_THM]
+  >> fs[] >> Cases_on `z` >> fs[]);
+
+val FIND_APPEND = Q.store_thm("FIND_APPEND",
+  `FIND f (l1 ++ l2) =
+   case FIND f l1 of NONE => FIND f l2
+      | SOME e => SOME e`,
+  Induct_on `l1` >> fs[FIND_def,INDEX_FIND_def]
+  >> rw[INDEX_FIND_normalize]);
+
+val FIND_NOT_MEM = Q.store_thm("FIND_NOT_MEM",
+  `!e l. FIND ($= e) l = NONE <=> ¬MEM e l`,
+  Induct_on `l` >> rw[FIND_def,INDEX_FIND_def] >> fs[FIND_def,INDEX_FIND_normalize']);
+
+val FIND_o_NOT_MEM = Q.store_thm("FIND_o_NOT_MEM",
+  `!e f l. FIND ($= e o f) l = NONE <=> ¬MEM e (MAP f l)`,
+  Induct_on `l` >> rw[FIND_def,INDEX_FIND_def] >> fs[FIND_def,INDEX_FIND_normalize']);
+
+val FIND_o_MEM = Q.store_thm("FIND_o_MEM",
+  `!e f l. FIND ($= e o f) l <> NONE <=> MEM e (MAP f l)`,
+  Induct_on `l` >> rw[FIND_def,INDEX_FIND_def] >> fs[FIND_def,INDEX_FIND_normalize']);
+
+val FIND_MEM = Q.store_thm("FIND_MEM",
+  `!f l z. FIND f l = SOME z
+   ==> MEM z l /\ f z`,
+  Induct_on `l` >> rpt strip_tac
+  >> fs[FIND_def,INDEX_FIND_def] >> every_case_tac
+  >> rveq >> fs[INDEX_FIND_normalize'' |> Q.SPEC `0` |> REWRITE_RULE [GSYM ONE]]
+  >> metis_tac[FST,SND]);
+
 val trans_enqueue' = Q.store_thm("trans_enqueue'",
   `∀s d p1 p2 e q.
      p1 ≠ p2
@@ -78,6 +124,38 @@ val trans_ext_choice_r' = Q.store_thm("trans_ext_choice_r'",
   >> match_mp_tac (trans_ext_choice_r)
   >> simp[]);
 
+val trans_ext_choice_F_receive = Q.store_thm("trans_ext_choice_F_receive",
+  `!e1 e2 p1 p2. trans e1 (LReceive p1 [0w] p2) e2 =
+           trans e1 (LExtChoice p1 F p2) e2
+  `,
+  `!e1 alpha e2. trans e1 alpha e2 ==>
+     !p1 p2. alpha = LReceive p1 [0w] p2 ==> trans e1 (LExtChoice p1 F p2) e2`
+  by(ho_match_mp_tac trans_ind
+     >> rpt strip_tac >> fs[] >> rveq >> fs[]
+     >> MAP_FIRST match_mp_tac (CONJUNCTS trans_rules) >> fs[])
+  >> `!e1 alpha e2. trans e1 alpha e2 ==>
+       !p1 p2. alpha = LExtChoice p1 F p2 ==> trans e1 (LReceive p1 [0w] p2) e2`
+    by(ho_match_mp_tac trans_ind
+       >> rpt strip_tac >> fs[] >> rveq >> fs[]
+       >> MAP_FIRST match_mp_tac (CONJUNCTS trans_rules) >> fs[])
+  >> rw[EQ_IMP_THM]);
+
+val trans_ext_choice_T_receive = Q.store_thm("trans_ext_choice_T_receive",
+  `!e1 e2 p1 p2. trans e1 (LReceive p1 [1w] p2) e2 =
+           trans e1 (LExtChoice p1 T p2) e2
+  `,
+  `!e1 alpha e2. trans e1 alpha e2 ==>
+     !p1 p2. alpha = LReceive p1 [1w] p2 ==> trans e1 (LExtChoice p1 T p2) e2`
+  by(ho_match_mp_tac trans_ind
+     >> rpt strip_tac >> fs[] >> rveq >> fs[]
+     >> MAP_FIRST match_mp_tac (CONJUNCTS trans_rules) >> fs[])
+  >> `!e1 alpha e2. trans e1 alpha e2 ==>
+       !p1 p2. alpha = LExtChoice p1 T p2 ==> trans e1 (LReceive p1 [1w] p2) e2`
+    by(ho_match_mp_tac trans_ind
+       >> rpt strip_tac >> fs[] >> rveq >> fs[]
+       >> MAP_FIRST match_mp_tac (CONJUNCTS trans_rules) >> fs[])
+  >> rw[EQ_IMP_THM]);
+
 val trans_IMP_weak_trans = Q.store_thm("trans_IMP_weak_trans",
   `∀ p alpha q. trans p alpha q ==> weak_trans p alpha q`,
   rw[weak_trans_def,weak_tau_trans_def]
@@ -137,6 +215,11 @@ val reduction_nil = Q.store_thm("reduction_nil",
   >> ho_match_mp_tac RTC_lifts_invariants
   >> simp[endpointSemanticsTheory.reduction_def,trans_nil_false]);
 
+val endpoints_def = Define `
+   (endpoints endpointLang$NNil = [])
+/\ (endpoints (NEndpoint p1 s e1) = [(p1,s,e1)])
+/\ (endpoints (NPar n1 n2) = endpoints n1 ++ endpoints n2)`
+
 val (junkcong_rules, junkcong_ind, junkcong_cases) = Hol_reln `
   (* Reflexive *)
   (∀fvs n:endpointLang$network. junkcong fvs n n)
@@ -194,6 +277,16 @@ val junkcong_add_junk'' = Q.store_thm("junkcong_add_junk''",
      by(unabbrev_all_tac >> simp[])
  >> rveq
  >> match_mp_tac junkcong_add_junk >> simp[]);
+
+val junkcong_add_junk''' = Q.store_thm("junkcong_add_junk'''",
+  `∀p s q e v fvs d.
+     v ∈ fvs ∧ ¬MEM v (free_var_names_endpoint e) ⇒
+     junkcong fvs (NEndpoint p (s with queue := q) e)
+     (NEndpoint p (s with <|bindings := s.bindings |+ (v,d); queue := q|>) e)`,
+  rpt strip_tac
+  >> qpat_abbrev_tac `a1 = s with queue := q`
+  >> `s.bindings = a1.bindings` by(unabbrev_all_tac >> simp[])
+  >> fs[junkcong_add_junk]);
 
 val junkcong_remove_junk = Q.store_thm("junkcong_remove_junk",
   `(∀p s e v fvs.
@@ -396,12 +489,64 @@ val junkcong_trans_eq = Q.store_thm("junkcong_trans_eq",
       >> imp_res_tac trans_par_r
       >> metis_tac[junkcong_rules]));
 
+val junkcong_has_fv_eq = Q.store_thm("junkcong_has_fv_eq",
+  `!fv e l s e2. junkcong {fv} (NEndpoint l s e) e2
+   /\ MEM fv (free_var_names_endpoint e)
+   ==> NEndpoint l s e = e2`,
+  `!fvs e1 e2. junkcong fvs e1 e2
+   ==> (!fv e l s. e1 = NEndpoint l s e /\ fvs = {fv} /\ MEM fv (free_var_names_endpoint e)
+                        ==> NEndpoint l s e = e2) /\
+       (!fv e l s. e2 = NEndpoint l s e /\ fvs = {fv} /\ MEM fv (free_var_names_endpoint e)
+                        ==> e1 = NEndpoint l s e)
+  ` suffices_by metis_tac[]
+  >> ho_match_mp_tac junkcong_strongind
+  >> rpt strip_tac
+  >> fs[] >> rveq >> fs[]);
+
+val junkcong_nil_rel_nil = Q.store_thm("junkcong_nil_rel_nil",
+  `!fvs n2.
+   junkcong fvs NNil n2 ==> n2 = NNil`,
+  `!fvs n1 n2.
+    junkcong fvs n1 n2
+    ==> (n1 = NNil <=> n2 = NNil)`
+    suffices_by metis_tac[]
+  >> ho_match_mp_tac junkcong_strongind
+  >> rpt strip_tac >> fs[]);
+
+val junkcong_par_rel_par = Q.store_thm("junkcong_par_rel_par",
+  `!fvs n1 n2 n3.
+   junkcong fvs (NPar n1 n2) n3 ==> ?n4 n5. n3 = NPar n4 n5 /\ junkcong fvs n1 n4 /\ junkcong fvs n2 n5`,
+  `!fvs n1 n2.
+    junkcong fvs n1 n2
+    ==> (!n3 n4. n1 = NPar n3 n4 ==> ?n5 n6. n2 = NPar n5 n6 /\ junkcong fvs n3 n5 /\ junkcong fvs n4 n6)
+        /\ (!n3 n4. n2 = NPar n3 n4 ==> ?n5 n6. n1 = NPar n5 n6 /\ junkcong fvs n5 n3 /\ junkcong fvs n6 n4)`
+    suffices_by metis_tac[]
+  >> ho_match_mp_tac junkcong_strongind
+  >> rpt strip_tac >> fs[junkcong_refl,junkcong_sym]
+  >> rfs[] >> fs[] >> metis_tac[junkcong_trans]);
+
+val junkcong_endpoint_rel_endpoint = Q.store_thm("junkcong_endpoint_rel_endpoint",
+  `!fvs p1 s1 e1 n2.
+   junkcong fvs (NEndpoint p1 s1 e1) n2 ==> ?s2. n2 = NEndpoint p1 s2 e1`,
+  `!fvs n1 n2.
+    junkcong fvs n1 n2
+    ==> (!p1 s1 e1. n1 = NEndpoint p1 s1 e1 ==> ?s2. n2 = NEndpoint p1 s2 e1)
+        /\ !p2 s2 e2. n2 = NEndpoint p2 s2 e2 ==> ?s1. n1 = NEndpoint p2 s1 e2`
+    suffices_by metis_tac[]
+  >> ho_match_mp_tac junkcong_strongind
+  >> rpt strip_tac >> fs[]);
+
+val junkcong_endpoints = Q.store_thm("junkcong_endpoints",
+  `!fvs n1 n2. junkcong fvs n1 n2 ==> MAP FST (endpoints n1) = MAP FST (endpoints n2)`,
+  ho_match_mp_tac junkcong_ind
+  >> rpt strip_tac >> fs[endpoints_def]);
+
 val junkcong_trans_pres = Q.store_thm("junkcong_trans_pres",
   `∀p1 q1 fv alpha p2.
      junkcong fv p1 q1 ∧ trans p1 alpha p2
      ⇒ ∃q2. trans q1 alpha q2 ∧ junkcong fv p2 q2`,
   metis_tac[junkcong_trans_eq])
-
+                                     
 val list_trans_def = Define `
     (list_trans p [] q = (p = q))
  /\ (list_trans p (alpha::l) q = ?p'. trans p alpha p' /\ list_trans p' l q)`
@@ -425,11 +570,6 @@ val list_trans_par_r = Q.store_thm("list_trans_par_r",
   >- simp[list_trans_def]
   >> rpt strip_tac
   >> fs[list_trans_def] >> metis_tac[endpointSemanticsTheory.trans_par_r]);
-
-val endpoints_def = Define `
-   (endpoints endpointLang$NNil = [])
-/\ (endpoints (NEndpoint p1 s e1) = [(p1,s,e1)])
-/\ (endpoints (NPar n1 n2) = endpoints n1 ++ endpoints n2)`
 
 val endpoint_names_trans = Q.store_thm("endpoint_names_trans",
   `!n1 alpha n2. trans n1 alpha n2 ==> MAP FST (endpoints n2) = MAP FST(endpoints n1)`,
@@ -486,5 +626,167 @@ val receiver_is_endpoint = Q.store_thm("receiver_is_endpoint",
   >> ho_match_mp_tac trans_strongind
   >> rpt strip_tac >> fs[] >> rveq
   >> fs[endpoints_def]);
+
+val free_names_are_names_endpoint = Q.store_thm("free_names_are_names_endpoint",
+  `!e v. MEM v (free_var_names_endpoint e) ==> MEM v (var_names_endpoint e)`,
+  Induct >> rpt strip_tac
+  >> fs[var_names_endpoint_def,free_var_names_endpoint_def,MEM_FILTER]);
+
+val free_names_are_names = Q.store_thm("free_names_are_names",
+  `!n v. MEM v (free_var_names_network n) ==> MEM v (var_names_network n)`,
+  Induct >> rpt strip_tac
+  >> fs[var_names_network_def,free_var_names_network_def,free_names_are_names_endpoint]);
+
+val trans_var_names_mono = Q.store_thm("trans_var_names_mono",
+  `!n1 alpha n2 fv.
+    trans n1 alpha n2
+    ∧ MEM fv (var_names_network n2) ==> MEM fv (var_names_network n1)`,
+  rpt strip_tac
+  >> qpat_x_assum `MEM _ _` mp_tac
+  >> MAP_EVERY (W(curry Q.SPEC_TAC)) [`fv`]
+  >> pop_assum mp_tac
+  >> MAP_EVERY (W(curry Q.SPEC_TAC)) [`n2`,`alpha`,`n1`]
+  >> ho_match_mp_tac trans_strongind
+  >> rpt strip_tac
+  >> fs[var_names_network_def,var_names_endpoint_def]);
+
+val partners_endpoint_def = Define `
+   (partners_endpoint Nil = [])
+∧ (partners_endpoint (Send p v e) = p::(partners_endpoint e))
+∧ (partners_endpoint (Receive p v e) = p::(partners_endpoint e))
+∧ (partners_endpoint (IntChoice b p e) =
+    p::(partners_endpoint e))
+∧ (partners_endpoint (ExtChoice p e1 e2) =
+    p::((partners_endpoint e1) ++ (partners_endpoint e2)))
+∧ (partners_endpoint (IfThen v e1 e2) = (partners_endpoint e1) ++ (partners_endpoint e2))
+∧ (partners_endpoint (Let v f vl e) = partners_endpoint e)`
+
+val partners_network_def = Define `
+   (partners_network NNil = [])
+∧ (partners_network (NPar n1 n2) = (partners_network n1 ++ partners_network n2))
+∧ (partners_network (NEndpoint p s e) = (partners_endpoint e))`
+
+val closed_under_def = Define `
+  closed_under s n = (set(partners_network n) ⊆ s)`
+
+val closed_network_def = Define `
+  closed_network n = closed_under (set(MAP FST (endpoints n))) n`
+
+val endpoint_ok_def = Define `
+  endpoint_ok (n,s,e) = ~MEM n (partners_endpoint e)`
+
+val weak_trans_refl = Q.store_thm("weak_trans_refl",
+  `!n. weak_trans n LTau n`,
+  rw[weak_trans_def]);
+
+val closed_under_junkcong = Q.store_thm("closed_under_junkcong",
+  `!fvs n1 n2 e. junkcong fvs n1 n2 /\ set (MAP FST (endpoints n1)) ⊆ e ==> closed_under e n1 = closed_under e n2`,
+  Induct_on `n1`
+  >> rpt strip_tac
+  >> imp_res_tac junkcong_endpoint_rel_endpoint
+  >> imp_res_tac junkcong_par_rel_par
+  >> imp_res_tac junkcong_nil_rel_nil
+  >> fs[closed_network_def] >> rveq >> fs[closed_under_def,partners_network_def,endpoints_def]
+  >> metis_tac[]);
+
+val closed_network_junkcong = Q.store_thm("closed_network_junkcong",
+  `!fvs n1 n2 e. junkcong fvs n1 n2 ==> closed_network n1 = closed_network n2`,
+  rpt strip_tac >> drule closed_under_junkcong
+  >> disch_then(qspec_then `set (MAP FST (endpoints n1))` mp_tac)
+  >> impl_tac >- MATCH_ACCEPT_TAC SUBSET_REFL
+  >> simp[closed_network_def] >> imp_res_tac junkcong_endpoints
+  >> rw[]);
+
+enval closed_under_receiver_mem = Q.store_thm("closed_under_receiver_mem",
+  `!n1 p1 d p2 n2 e.
+     trans n1 (LSend p1 d p2) n2 /\ closed_under e n1
+      /\ set (MAP FST (endpoints n1)) ⊆ e
+     ==> p2 ∈ e
+  `,
+  rpt strip_tac
+  >> ntac 2 (pop_assum mp_tac)
+  >> qmatch_asmsub_abbrev_tac `trans _ a1 _`
+  >> pop_assum (mp_tac o PURE_ONCE_REWRITE_RULE [markerTheory.Abbrev_def])
+  >> MAP_EVERY (W(curry Q.SPEC_TAC)) [`p1`,`p2`,`d`,`e`]
+  >> pop_assum mp_tac
+  >> MAP_EVERY (W(curry Q.SPEC_TAC)) [`n2`,`a1`,`n1`]
+  >> ho_match_mp_tac trans_strongind
+  >> rpt strip_tac >> fs[] >> rveq
+  >> fs[endpoints_def,closed_under_def,partners_endpoint_def,partners_network_def]);
+
+val closed_network_receiver_mem = Q.store_thm("closed_network_receiver_mem",
+  `!n1 p1 d p2 n2 e.
+     trans n1 (LSend p1 d p2) n2 /\ closed_network n1
+     ==> MEM p2 (MAP FST (endpoints n1))
+  `,
+  rpt strip_tac
+  >> fs[closed_network_def]
+  >> imp_res_tac closed_under_receiver_mem
+  >> fs[]);
+
+val var_names_endpoint_in_network = Q.store_thm("var_names_endpoint_in_network",
+  `!fv e n. MEM fv (var_names_endpoint (SND(SND(e))))
+            /\ MEM e (endpoints n) ==> MEM fv (var_names_network n)`,
+  Induct_on `n` >> rpt strip_tac >> fs[var_names_network_def,endpoints_def]
+  >> metis_tac[]);
+
+val free_var_names_endpoint_in_network = Q.store_thm("free_var_names_endpoint_in_network",
+  `!fv e n. MEM fv (free_var_names_endpoint (SND(SND(e))))
+            /\ MEM e (endpoints n) ==> MEM fv (free_var_names_network n)`,
+  Induct_on `n` >> rpt strip_tac >> fs[free_var_names_network_def,endpoints_def]
+  >> metis_tac[]);
+
+val endpoint_names_reduction = Q.store_thm("endpoint_names_reduction",
+  `!n1 n2. reduction^* n1 n2 ==> MAP FST (endpoints n2) = MAP FST (endpoints n1)`,
+  PURE_ONCE_REWRITE_TAC[EQ_SYM_EQ]
+  >> ho_match_mp_tac RTC_lifts_reflexive_transitive_relations
+  >> rpt strip_tac >> fs[reduction_def] >> imp_res_tac endpoint_names_trans
+  >> fs[reflexive_def,transitive_def]);
+
+val junkcong_var_names = Q.store_thm("junkcong_var_names",
+  `!fvs n1 n2. junkcong fvs n1 n2 ==> var_names_network n1 = var_names_network n2`,
+  ho_match_mp_tac junkcong_ind >> rpt strip_tac
+  >> fs[var_names_network_def]);
+
+val junkcong_free_var_names = Q.store_thm("junkcong_free_var_names",
+  `!fvs n1 n2. junkcong fvs n1 n2 ==> free_var_names_network n1 = free_var_names_network n2`,
+  ho_match_mp_tac junkcong_ind >> rpt strip_tac
+  >> fs[free_var_names_network_def]);
+
+val trans_endpoints_ok = Q.store_thm("trans_endpoints_ok",
+  `!n1 alpha n2. trans n1 alpha n2
+                 ==> EVERY endpoint_ok (endpoints n1)
+                 ==> EVERY endpoint_ok (endpoints n2)`,
+  ho_match_mp_tac trans_ind
+  >> rpt strip_tac
+  >> fs[endpoints_def,endpoint_ok_def,partners_endpoint_def]);
+
+val reduction_endpoints_ok = Q.store_thm("reduction_endpoints_ok",
+  `!n1 n2. reduction^* n1 n2 /\ EVERY endpoint_ok (endpoints n1)
+                 ==> EVERY endpoint_ok (endpoints n2)`,
+  PURE_ONCE_REWRITE_TAC [CONJ_SYM]
+  >> ho_match_mp_tac RTC_lifts_invariants
+  >> metis_tac[trans_endpoints_ok,reduction_def]);
+
+val closed_under_trans = Q.store_thm("closed_under_trans",
+  `!n1 alpha n2 e. trans n1 alpha n2 /\ closed_under e n1 ==> closed_under e n2`,
+  simp[GSYM AND_IMP_INTRO,RIGHT_FORALL_IMP_THM]
+  >> ho_match_mp_tac trans_ind
+  >> rpt strip_tac >> fs[closed_under_def,partners_network_def,partners_endpoint_def]);
+
+val closed_network_trans = Q.store_thm("closed_network_trans",
+  `!n1 alpha n2. trans n1 alpha n2 /\ closed_network n1 ==> closed_network n2`,
+  rpt strip_tac
+  >> fs[closed_network_def]
+  >> imp_res_tac endpoint_names_trans
+  >> fs[]
+  >> imp_res_tac closed_under_trans);
+
+val closed_network_reduction = Q.store_thm("closed_network_reduction",
+  `!n1 n2. reduction^* n1 n2 /\ closed_network n1 ==> closed_network n2`,
+  simp[Once CONJ_SYM]
+  >> ho_match_mp_tac RTC_lifts_invariants
+  >> simp[Once CONJ_SYM, reduction_def]
+  >> MATCH_ACCEPT_TAC closed_network_trans);
 
 val _ = export_theory ()
